src/Init/Data/List/Basic.lean
@@ -225,10 +225,23 @@ def lex [BEq α] (l₁ l₂ : List α) (lt : α → α → Bool := by exact (· 
   | _,      []       => false
   | a :: as, b :: bs => lt a b || (a == b && lex as bs lt)
 
-@[simp] theorem lex_nil_nil [BEq α] : lex ([] : List α) [] lt = false := rfl
-@[simp] theorem lex_nil_cons [BEq α] {b} {bs : List α} : lex [] (b :: bs) lt = true := rfl
-@[simp] theorem lex_cons_nil [BEq α] {a} {as : List α} : lex (a :: as) [] lt = false := rfl
-@[simp] theorem lex_cons_cons [BEq α] {a b} {as bs : List α} :
+theorem nil_lex_nil [BEq α] : lex ([] : List α) [] lt = false := rfl
+@[simp] theorem nil_lex_cons [BEq α] {b} {bs : List α} : lex [] (b :: bs) lt = true := rfl
+theorem cons_lex_nil [BEq α] {a} {as : List α} : lex (a :: as) [] lt = false := rfl
+@[simp] theorem cons_lex_cons [BEq α] {a b} {as bs : List α} :
+    lex (a :: as) (b :: bs) lt = (lt a b || (a == b && lex as bs lt)) := rfl
+
+@[simp] theorem lex_nil [BEq α] {as : List α} : lex as [] lt = false := by
+  cases as <;> simp [nil_lex_nil, cons_lex_nil]
+
+@[deprecated nil_lex_nil (since := "2025-02-10")]
+theorem lex_nil_nil [BEq α] : lex ([] : List α) [] lt = false := rfl
+@[deprecated nil_lex_cons (since := "2025-02-10")]
+theorem lex_nil_cons [BEq α] {b} {bs : List α} : lex [] (b :: bs) lt = true := rfl
+@[deprecated cons_lex_nil (since := "2025-02-10")]
+theorem lex_cons_nil [BEq α] {a} {as : List α} : lex (a :: as) [] lt = false := rfl
+@[deprecated cons_lex_cons (since := "2025-02-10")]
+theorem lex_cons_cons [BEq α] {a b} {as bs : List α} :
     lex (a :: as) (b :: bs) lt = (lt a b || (a == b && lex as bs lt)) := rfl
 
 /-! ## Alternative getters -/
